fp_inv

bls12-381_coq/bls.v
@@ -12,6 +12,7 @@ From Coq Require Import ZArith.
 Require Import List. Import ListNotations.
 Open Scope hacspec_scope.
 Open Scope bool_scope.
+From Coqprime Require Import GZnZ.
 
 Notation "a >?? b" := (Nat.ltb b a) (at level 79).
 
@@ -89,14 +90,46 @@ Definition fp_one := one.
 Definition fp_two := repr 2.
 Definition fp_exp (x y : int) := repr (Z.pow (unsigned x) (unsigned y)).
 
-Axiom fp_inv : int -> int.
-Axiom fp_inv_is_multiplicative_inverse : forall (n : int), mul n (fp_inv n) = one.
+Definition prime := 0x1a0111ea397fe69a4b1ba7b6434bacd764774b84f38512bf6730d2a0f6b0f6241eabfffeb153ffffb9feffffffffaaab%Z.
+
+Definition fp_inv a: int := repr (val prime (inv prime (mkznz prime _ (modz prime (unsigned a))))).
+
+Lemma helper4: forall a: Z, (0 <= a < prime)%Z -> a = val prime (mkznz prime _ (modz prime a)).
+Proof. intros a H. simpl. symmetry. apply (Z.mod_small). apply H.
+Qed.
+Check GZnZ.mul.
+
+Lemma helper6: modulus = prime.
+Proof. compute. Admitted.
+
+Lemma helper5: forall (a: Z) (b: znz prime), (0 <= a < prime)%Z -> repr (a * (val prime b)) = repr (val prime (GZnZ.mul prime (mkznz prime _ (modz prime a)) b)).
+Proof. intros a b H. apply eqm_samerepr. simpl. rewrite (Z.mod_small a).  unfold eqm. rewrite helper6. apply Zbits.eqmod_mod. reflexivity. apply H.
+Qed.
+
+Lemma helper7: forall a, (0 <= val prime a < prime)%Z.
+Proof. intro a. destruct a. simpl. rewrite inZnZ. apply Z.mod_pos_bound. reflexivity. 
+Qed.
+
+Require Import Blsprime.blsprime.
+
+Lemma fp_inv_is_multiplicative_inverse : forall (n : int), n <> fp_zero -> mul n (fp_inv n) = one.
+Proof. intros n H. unfold mul. unfold fp_inv. rewrite unsigned_repr_eq. generalize (FZpZ prime blsprime). intros H1. destruct H1. destruct F_R.
+  rewrite Z.mod_small.
+  - rewrite helper5. rewrite Rmul_comm. rewrite Finv_l. 
+    + reflexivity.
+    + intro c. destruct H. inversion c. apply eqm_refl2 in H0. apply eqm_samerepr in H0. rewrite (Z.mod_small) in H0. rewrite (Z.mod_small) in H0. rewrite repr_unsigned in H0. rewrite H0. reflexivity.
+      split; reflexivity.
+      generalize (unsigned_range n). intro he. rewrite helper6 in he. apply he.
+    + generalize (unsigned_range n). intro he. rewrite helper6 in he. apply he.
+  - rewrite helper6. apply helper7.
+Qed.
+
 
 Definition fp_div a b: fp := a * (fp_inv b) .
 
 
 Example test1 : mul fp_two (fp_inv fp_two) = fp_one. (* This should be "inv 1 = 1"*)
-Proof. apply fp_inv_is_multiplicative_inverse. Qed.
+Proof. apply fp_inv_is_multiplicative_inverse. intro c. discriminate c. Qed.
 
 
 Definition fp2fromfp (n_2 : fp) : fp2 :=
@@ -756,7 +789,7 @@ Proof. split.
 - apply fp_ring_theory.
 - unfold fp_eq. unfold "<>". intros H. discriminate.
 - reflexivity.
-- intro x. unfold fp_eq. intros H. rewrite mul_commut. apply fp_inv_is_multiplicative_inverse.
+- intro x. unfold fp_eq. intros H. rewrite mul_commut. apply (fp_inv_is_multiplicative_inverse x H).
 Qed.
 
 Add Field fp_field: fp_field_theory.
@@ -887,10 +920,10 @@ Proof. intros x1 y1 x2 y2 H1 H2 H3. generalize (nonzero_iff (y1 + y2) (y1 - y2))
   - intros contra. destruct contra. reflexivity.
 Qed.
 
-(* Admitted because weird compilation *)
+(* Admitted because weird compilation (wprdsize is weird) *)
 Lemma exp2ismul: forall x, fp_exp x (pub_u32 2) = x * x.
-Proof. intros x. unfold fp_exp. unfold unsigned. unfold intval. rewrite N_to_int2. simpl. destruct x as (a,p).
-  simpl. unfold Zbits.P_mod_two_p.  
+Proof. intros x. unfold fp_exp. unfold Z.pow. unfold unsigned. unfold intval. rewrite N_to_int2. simpl. destruct x as (a,p).
+  simpl. unfold Zbits.P_mod_two_p. simpl.  
 Admitted.
 
 
@@ -998,4 +1031,4 @@ Proof. split.
   intros H1; destruct H; apply helper1 in H1; destruct H1; rewrite H0; rewrite H; apply pair_equal_spec; split; reflexivity.
 Qed.
 
-Add Field fp_field: fp_field_theory.
+Add Field fp2_field: fp2_field_theory.
